LeanGrow/F/Prototypes/MarkThree/Frontend.lean
@@ -92,7 +92,7 @@ elab "grow" : tactic => do
     let premises :=(Names_to_thmData dEnv [`myAdd_zero, `Eq.trans].reverse)
     let st : SearchState := ⟨⟨0,1,0,[(0,goal)], .ofGoal 0 goal [] [] [] ⟩, ltx, forw2, (fun x => (x / 42, x % 42)), ltx.length, fctx, [], [], [],[],[]⟩
     --logInfoAt ref s!"{repr premises}"
-    let res := search 5 premises st
+    let res := search 20 premises st
     match res with
     | .none => logInfoAt ref "nope"
     | .some res! => logInfoAt ref s!"Recovered : {repr res!}"
